Forward_simulation almost completed.

backend/ValueAnalysis.v
@@ -885,7 +885,6 @@ Qed.
 
 (** Construction 6: external call *)
 
-(* REDACTED
 Theorem external_call_match:
   forall ef (ge: genv) vargs m t vres m' bc rm am,
   external_call ef ge vargs m t vres m' ->
@@ -906,12 +905,11 @@ Theorem external_call_match:
 Proof.
   intros until am; intros EC GENV ARGS RO MM NOSTACK.
   (* Part 1: using ec_mem_inject *)
-  exploit (@external_call_mem_inject ef _ _ ge vargs m t vres m' (inj_of_bc bc) m vargs).
+  exploit (@external_call_mem_inject' ef _ _ ge vargs m t vres m' (inj_of_bc bc) m vargs).
   apply inj_of_bc_preserves_globals; auto.
   exact EC.
   eapply mmatch_inj; eauto. eapply mmatch_below; eauto.
   revert ARGS. generalize vargs.
-  { (*PROBLEM*) intros. intros b HH.
   induction vargs0; simpl; intros; constructor.
   eapply vmatch_inj; eauto. auto.
   intros (j' & vres' & m'' & t' & EC' & IRES & IMEM & UNCH1 & UNCH2 & IINCR & ISEP & INJT).
@@ -1017,7 +1015,7 @@ Proof.
   intros. eapply Mem.loadbytes_unchanged_on_1; auto.
   apply UNCH1; auto. intros; red. unfold inj_of_bc; rewrite H0; auto.
 Qed.
-*)
+
 Remark list_forall2_in_l:
   forall (A B: Type) (P: A -> B -> Prop) x1 l1 l2,
   list_forall2 P l1 l2 -> In x1 l1 -> exists x2, In x2 l2 /\ P x1 x2.
@@ -1217,7 +1215,7 @@ Proof.
   econstructor; eauto.
 Qed.
 
-(*Theorem sound_step_base:
+Theorem sound_step_base:
   forall st t st', RTL.step ge st t st' -> sound_state_base st -> sound_state_base st'.
 Proof.
   induction 1; intros SOUND; inv SOUND.
@@ -1464,7 +1462,7 @@ Proof.
    eapply sound_regular_state with (bc := bc1); eauto.
    apply sound_stack_exten with bc'; auto.
    eapply ematch_ge; eauto. apply ematch_update. auto. auto.
-Qed. *)
+Qed.
 
 End SOUNDNESS.
 
@@ -1479,13 +1477,16 @@ Section LINKING.
 Variable prog: program.
 Let ge := Genv.globalenv prog.
 
-Definition sound_state: state -> Prop := fun s =>  True.
-(*
+Inductive sound_state: state -> Prop :=
+  | sound_state_intro: forall st,
+      (forall cunit, linkorder cunit prog -> sound_state_base cunit ge st) ->
+      sound_state st.
+
 Theorem sound_step:
   forall st t st', RTL.step ge st t st' -> sound_state st -> sound_state st'.
 Proof.
   intros. inv H0. constructor; intros. eapply sound_step_base; eauto. 
-Qed.*)
+Qed.
 
 Remark sound_state_inv:
   forall st cunit,
