driver/Compiler.v
@@ -15,7 +15,7 @@
 (** Libraries. *)
 Require Import String.
 Require Import Coqlib Errors.
-Require Import AST Linking Smallstep.
+Require Import AST Linking Smallstep ExposedSmallstep2.
 (** Languages (syntax and semantics). *)
 Require Ctypes Csyntax Csem Cstrategy Cexec.
 Require Clight.
@@ -40,7 +40,7 @@ Require Inlining.
 Require Renumber.
 Require Constprop.
 Require CSE.
-Require Deadcode.
+Require Deadcode. 
 Require Unusedglob.
 Require Allocation.
 Require Tunneling.
@@ -51,24 +51,25 @@ Require Stacking.
 Require Asmgen.
 (** Proofs of semantic preservation. *)
 Require SimplExprproof.
-Require SimplLocalsproof.
+(*Require SimplLocalsproof.*)
 Require Cshmgenproof.
 Require Cminorgenproof.
 Require Selectionproof.
 Require RTLgenproof.
 Require Tailcallproof.
-Require Inliningproof.
+(*Require Inliningproof.*)
 Require Renumberproof.
 Require Constpropproof.
 Require CSEproof.
 Require Deadcodeproof.
-Require Unusedglobproof.
+(*Require Unusedglobproof.*)
 Require Allocproof.
 Require Tunnelingproof.
 Require Linearizeproof.
 Require CleanupLabelsproof.
 Require Debugvarproof.
-Require Stackingproof.
+Require Stackingproof_temp.
+(*Require Stackingproof.*)
 Require Asmgenproof.
 (** Command-line flags. *)
 Require Import Compopts.
@@ -117,12 +118,10 @@ Definition partial_if {A: Type}
   RTL program.  The three translations produce Asm programs ready for
   pretty-printing and assembling. *)
 
-Definition transf_rtl_program (f: RTL.program) : res Asm.program :=
-   OK f
+Definition simpl_transf_rtl_program (f: RTL.program) : res Asm.program:=
+  OK f
    @@ print (print_RTL 0)
    @@ total_if Compopts.optim_tailcalls (time "Tail calls" Tailcall.transf_program)
-   @@ print (print_RTL 1)
-  @@@ time "Inlining" Inlining.transf_program
    @@ print (print_RTL 2)
    @@ time "Renumbering" Renumber.transf_program
    @@ print (print_RTL 3)
@@ -130,11 +129,11 @@ Definition transf_rtl_program (f: RTL.program) : res Asm.program :=
    @@ print (print_RTL 4)
    @@ total_if Compopts.optim_constprop (time "Renumbering" Renumber.transf_program)
    @@ print (print_RTL 5)
-  @@@ partial_if Compopts.optim_CSE (time "CSE" CSE.transf_program)
+  @@@ partial_if Compopts.optim_CSE (time "CSE" CSE.transf_program)(*
    @@ print (print_RTL 6)
-  @@@ partial_if Compopts.optim_redundancy (time "Redundancy elimination" Deadcode.transf_program)
+  @@@ partial_if Compopts.optim_redundancy (time "Redundancy elimination" Deadcode.transf_program) *)(*
    @@ print (print_RTL 7)
-  @@@ time "Unused globals" Unusedglob.transform_program
+  @@@ time "Unused globals" Unusedglob.transform_program*)
    @@ print (print_RTL 8)
   @@@ time "Register allocation" Allocation.transf_program
    @@ print print_LTL
@@ -146,32 +145,19 @@ Definition transf_rtl_program (f: RTL.program) : res Asm.program :=
    @@ print print_Mach
   @@@ time "Asm generation" Asmgen.transf_program.
 
-Definition transf_cminor_program (p: Cminor.program) : res Asm.program :=
+Definition simpl_transf_cminor_program (p: Cminor.program) : res Asm.program :=
    OK p
    @@ print print_Cminor
   @@@ time "Instruction selection" Selection.sel_program
   @@@ time "RTL generation" RTLgen.transl_program
-  @@@ transf_rtl_program.
-
-Definition transf_clight_program (p: Clight.program) : res Asm.program :=
-  OK p
-   @@ print print_Clight
-  @@@ time "Simplification of locals" SimplLocals.transf_program
-  @@@ time "C#minor generation" Cshmgen.transl_program
-  @@@ time "Cminor generation" Cminorgen.transl_program
-  @@@ transf_cminor_program.
+  @@@ simpl_transf_rtl_program.
 
 Definition simpl_transf_clight_program (p: Clight.program) : res Asm.program :=
   OK p
    @@ print print_Clight
   @@@ time "C#minor generation" Cshmgen.transl_program
   @@@ time "Cminor generation" Cminorgen.transl_program
-  @@@ transf_cminor_program.
-
-Definition transf_c_program (p: Csyntax.program) : res Asm.program :=
-  OK p
-  @@@ time "Clight generation" SimplExpr.transl_program
-  @@@ transf_clight_program.
+  @@@ simpl_transf_cminor_program.
 
 (** Force [Initializers] and [Cexec] to be extracted as well. *)
 
@@ -235,59 +221,31 @@ Qed.
 
 Local Open Scope linking_scope.
 
-Definition CompCert's_passes :=
-      mkpass SimplExprproof.match_prog
-  ::: mkpass SimplLocalsproof.match_prog
-  ::: mkpass Cshmgenproof.match_prog
-  ::: mkpass Cminorgenproof.match_prog
-  ::: mkpass Selectionproof.match_prog
-  ::: mkpass RTLgenproof.match_prog
-  ::: mkpass (match_if Compopts.optim_tailcalls Tailcallproof.match_prog)
-  ::: mkpass Inliningproof.match_prog
-  ::: mkpass Renumberproof.match_prog
-  ::: mkpass (match_if Compopts.optim_constprop Constpropproof.match_prog)
-  ::: mkpass (match_if Compopts.optim_constprop Renumberproof.match_prog)
-  ::: mkpass (match_if Compopts.optim_CSE CSEproof.match_prog)
-  ::: mkpass (match_if Compopts.optim_redundancy Deadcodeproof.match_prog)
-  ::: mkpass Unusedglobproof.match_prog
-  ::: mkpass Allocproof.match_prog
-  ::: mkpass Tunnelingproof.match_prog
-  ::: mkpass Linearizeproof.match_prog
-  ::: mkpass CleanupLabelsproof.match_prog
-  ::: mkpass (match_if Compopts.debug Debugvarproof.match_prog)
-  ::: mkpass Stackingproof.match_prog
-  ::: mkpass Asmgenproof.match_prog
-  ::: pass_nil _.
-
+Axiom Stackingproof_match_prog: Linear.program -> Mach.program -> Prop.
 
 Definition Simpl_CompCert's_passes :=
-      mkpass Cshmgenproof.match_prog
+   mkpass Cshmgenproof.match_prog
   ::: mkpass Cminorgenproof.match_prog
   ::: mkpass Selectionproof.match_prog
   ::: mkpass RTLgenproof.match_prog
   ::: mkpass (match_if Compopts.optim_tailcalls Tailcallproof.match_prog)
-  ::: mkpass Inliningproof.match_prog
   ::: mkpass Renumberproof.match_prog
   ::: mkpass (match_if Compopts.optim_constprop Constpropproof.match_prog)
   ::: mkpass (match_if Compopts.optim_constprop Renumberproof.match_prog)
   ::: mkpass (match_if Compopts.optim_CSE CSEproof.match_prog)
-  ::: mkpass (match_if Compopts.optim_redundancy Deadcodeproof.match_prog)
-  ::: mkpass Unusedglobproof.match_prog
   ::: mkpass Allocproof.match_prog
   ::: mkpass Tunnelingproof.match_prog
   ::: mkpass Linearizeproof.match_prog
   ::: mkpass CleanupLabelsproof.match_prog
   ::: mkpass (match_if Compopts.debug Debugvarproof.match_prog)
-  ::: mkpass Stackingproof.match_prog
+  ::: mkpass Stackingproof_temp.match_prog
   ::: mkpass Asmgenproof.match_prog
   ::: pass_nil _.
+
 
 (** Composing the [match_prog] relations above, we obtain the relation
   between CompCert C sources and Asm code that characterize CompCert's
   compilation. *)
-
-Definition match_prog: Csyntax.program -> Asm.program -> Prop :=
-  pass_match (compose_passes CompCert's_passes).
 
 Definition simpl_match_prog: Clight.program -> Asm.program -> Prop :=
   pass_match (compose_passes Simpl_CompCert's_passes).
@@ -305,100 +263,37 @@ Proof.
   rewrite ! compose_print_identity in T. simpl in T.
   destruct (Cshmgen.transl_program p) as [p3|e] eqn:P3; simpl in T; try discriminate.
   destruct (Cminorgen.transl_program p3) as [p4|e] eqn:P4; simpl in T; try discriminate.
-  unfold transf_cminor_program, time in T. rewrite ! compose_print_identity in T. simpl in T.
+  unfold simpl_transf_cminor_program, time in T. rewrite ! compose_print_identity in T. simpl in T.
   destruct (Selection.sel_program p4) as [p5|e] eqn:P5; simpl in T; try discriminate.
   destruct (RTLgen.transl_program p5) as [p6|e] eqn:P6; simpl in T; try discriminate.
-  unfold transf_rtl_program, time in T. rewrite ! compose_print_identity in T. simpl in T.
+  unfold simpl_transf_rtl_program, time in T. rewrite ! compose_print_identity in T. simpl in T.
   set (p7 := total_if optim_tailcalls Tailcall.transf_program p6) in *.
-  destruct (Inlining.transf_program p7) as [p8|e] eqn:P8; simpl in T; try discriminate.
-  set (p9 := Renumber.transf_program p8) in *.
-  set (p10 := total_if optim_constprop Constprop.transf_program p9) in *.
-  set (p11 := total_if optim_constprop Renumber.transf_program p10) in *.
-  destruct (partial_if optim_CSE CSE.transf_program p11) as [p12|e] eqn:P12; simpl in T; try discriminate.
-  destruct (partial_if optim_redundancy Deadcode.transf_program p12) as [p13|e] eqn:P13; simpl in T; try discriminate.
-  destruct (Unusedglob.transform_program p13) as [p14|e] eqn:P14; simpl in T; try discriminate.
-  destruct (Allocation.transf_program p14) as [p15|e] eqn:P15; simpl in T; try discriminate.
-  set (p16 := Tunneling.tunnel_program p15) in *.
-  destruct (Linearize.transf_program p16) as [p17|e] eqn:P17; simpl in T; try discriminate.
-  set (p18 := CleanupLabels.transf_program p17) in *.
-  destruct (partial_if debug Debugvar.transf_program p18) as [p19|e] eqn:P19; simpl in T; try discriminate.
-  destruct (Stacking.transf_program p19) as [p20|e] eqn:P20; simpl in T; try discriminate.
-  unfold match_prog; simpl. 
+  set (p8 := Renumber.transf_program p7) in *.
+  set (p9 := total_if optim_constprop Constprop.transf_program p8) in *.
+  set (p10 := total_if optim_constprop Renumber.transf_program p9) in *.
+  destruct (partial_if optim_CSE CSE.transf_program p10) as [p11|e] eqn:P11; simpl in T; try discriminate.
+  destruct (Allocation.transf_program p11) as [p12|e] eqn:P12; simpl in T; try discriminate.
+  set (p13 := Tunneling.tunnel_program p12) in *.
+  destruct (Linearize.transf_program p13) as [p14|e] eqn:P14; simpl in T; try discriminate.
+  set (p15 := CleanupLabels.transf_program p14) in *.
+  destruct (partial_if debug Debugvar.transf_program p15) as [p16|e] eqn:P16; simpl in T; try discriminate.
+  destruct (Stacking.transf_program p16) as [p17|e] eqn:P17; simpl in T; try discriminate.
+  unfold simpl_match_prog; simpl. 
   exists p3; split. apply Cshmgenproof.transf_program_match; auto.
   exists p4; split. apply Cminorgenproof.transf_program_match; auto.
   exists p5; split. apply Selectionproof.transf_program_match; auto.
   exists p6; split. apply RTLgenproof.transf_program_match; auto.
   exists p7; split. apply total_if_match. apply Tailcallproof.transf_program_match.
-  exists p8; split. apply Inliningproof.transf_program_match; auto.
-  exists p9; split. apply Renumberproof.transf_program_match; auto.
-  exists p10; split. apply total_if_match. apply Constpropproof.transf_program_match.
-  exists p11; split. apply total_if_match. apply Renumberproof.transf_program_match.
-  exists p12; split. eapply partial_if_match; eauto. apply CSEproof.transf_program_match.
-  exists p13; split. eapply partial_if_match; eauto. apply Deadcodeproof.transf_program_match.
-  exists p14; split. apply Unusedglobproof.transf_program_match; auto.
-  exists p15; split. apply Allocproof.transf_program_match; auto.
-  exists p16; split. apply Tunnelingproof.transf_program_match.
-  exists p17; split. apply Linearizeproof.transf_program_match; auto.
-  exists p18; split. apply CleanupLabelsproof.transf_program_match; auto.
-  exists p19; split. eapply partial_if_match; eauto. apply Debugvarproof.transf_program_match.
-  exists p20; split. apply Stackingproof.transf_program_match; auto.
-  exists tp; split. apply Asmgenproof.transf_program_match; auto. 
-  reflexivity.
-Qed.
-
-
-
-Theorem transf_c_program_match:
-  forall p tp,
-  transf_c_program p = OK tp ->
-  match_prog p tp.
-Proof.
-  intros p tp T.
-  unfold transf_c_program, time in T. simpl in T.
-  destruct (SimplExpr.transl_program p) as [p1|e] eqn:P1; simpl in T; try discriminate.
-  unfold transf_clight_program, time in T. rewrite ! compose_print_identity in T. simpl in T.
-  destruct (SimplLocals.transf_program p1) as [p2|e] eqn:P2; simpl in T; try discriminate.
-  destruct (Cshmgen.transl_program p2) as [p3|e] eqn:P3; simpl in T; try discriminate.
-  destruct (Cminorgen.transl_program p3) as [p4|e] eqn:P4; simpl in T; try discriminate.
-  unfold transf_cminor_program, time in T. rewrite ! compose_print_identity in T. simpl in T.
-  destruct (Selection.sel_program p4) as [p5|e] eqn:P5; simpl in T; try discriminate.
-  destruct (RTLgen.transl_program p5) as [p6|e] eqn:P6; simpl in T; try discriminate.
-  unfold transf_rtl_program, time in T. rewrite ! compose_print_identity in T. simpl in T.
-  set (p7 := total_if optim_tailcalls Tailcall.transf_program p6) in *.
-  destruct (Inlining.transf_program p7) as [p8|e] eqn:P8; simpl in T; try discriminate.
-  set (p9 := Renumber.transf_program p8) in *.
-  set (p10 := total_if optim_constprop Constprop.transf_program p9) in *.
-  set (p11 := total_if optim_constprop Renumber.transf_program p10) in *.
-  destruct (partial_if optim_CSE CSE.transf_program p11) as [p12|e] eqn:P12; simpl in T; try discriminate.
-  destruct (partial_if optim_redundancy Deadcode.transf_program p12) as [p13|e] eqn:P13; simpl in T; try discriminate.
-  destruct (Unusedglob.transform_program p13) as [p14|e] eqn:P14; simpl in T; try discriminate.
-  destruct (Allocation.transf_program p14) as [p15|e] eqn:P15; simpl in T; try discriminate.
-  set (p16 := Tunneling.tunnel_program p15) in *.
-  destruct (Linearize.transf_program p16) as [p17|e] eqn:P17; simpl in T; try discriminate.
-  set (p18 := CleanupLabels.transf_program p17) in *.
-  destruct (partial_if debug Debugvar.transf_program p18) as [p19|e] eqn:P19; simpl in T; try discriminate.
-  destruct (Stacking.transf_program p19) as [p20|e] eqn:P20; simpl in T; try discriminate.
-  unfold match_prog; simpl. 
-  exists p1; split. apply SimplExprproof.transf_program_match; auto.
-  exists p2; split. apply SimplLocalsproof.match_transf_program; auto.
-  exists p3; split. apply Cshmgenproof.transf_program_match; auto.
-  exists p4; split. apply Cminorgenproof.transf_program_match; auto.
-  exists p5; split. apply Selectionproof.transf_program_match; auto.
-  exists p6; split. apply RTLgenproof.transf_program_match; auto.
-  exists p7; split. apply total_if_match. apply Tailcallproof.transf_program_match.
-  exists p8; split. apply Inliningproof.transf_program_match; auto.
-  exists p9; split. apply Renumberproof.transf_program_match; auto.
-  exists p10; split. apply total_if_match. apply Constpropproof.transf_program_match.
-  exists p11; split. apply total_if_match. apply Renumberproof.transf_program_match.
-  exists p12; split. eapply partial_if_match; eauto. apply CSEproof.transf_program_match.
-  exists p13; split. eapply partial_if_match; eauto. apply Deadcodeproof.transf_program_match.
-  exists p14; split. apply Unusedglobproof.transf_program_match; auto.
-  exists p15; split. apply Allocproof.transf_program_match; auto.
-  exists p16; split. apply Tunnelingproof.transf_program_match.
-  exists p17; split. apply Linearizeproof.transf_program_match; auto.
-  exists p18; split. apply CleanupLabelsproof.transf_program_match; auto.
-  exists p19; split. eapply partial_if_match; eauto. apply Debugvarproof.transf_program_match.
-  exists p20; split. apply Stackingproof.transf_program_match; auto.
+  exists p8; split. apply Renumberproof.transf_program_match; auto.
+  exists p9; split. apply total_if_match. apply Constpropproof.transf_program_match.
+  exists p10; split. apply total_if_match. apply Renumberproof.transf_program_match.
+  exists p11; split. eapply partial_if_match; eauto. apply CSEproof.transf_program_match.
+  exists p12; split. apply Allocproof.transf_program_match; auto.
+  exists p13; split. apply Tunnelingproof.transf_program_match.
+  exists p14; split. apply Linearizeproof.transf_program_match; auto.
+  exists p15; split. apply CleanupLabelsproof.transf_program_match; auto.
+  exists p16; split. eapply partial_if_match; eauto. apply Debugvarproof.transf_program_match.
+  exists p17; split. apply Stackingproof_temp.transf_program_match; auto.
   exists tp; split. apply Asmgenproof.transf_program_match; auto. 
   reflexivity.
 Qed.
@@ -427,6 +322,18 @@ Proof.
 - subst s2. exists s1'; auto.
 Qed.
 
+Remark forward_injection_identity:
+  forall sem get_mem, forward_injection sem sem get_mem get_mem.
+Proof.
+  intros. econstructor.
+Admitted.
+
+Remark forward_extension_identity:
+  forall sem get_mem, forward_extension sem sem get_mem get_mem.
+Proof.
+  intros. econstructor.
+Admitted.
+
 Lemma match_if_simulation:
   forall (A: Type) (sem: A -> semantics) (flag: unit -> bool) (transf: A -> A -> Prop) (prog tprog: A),
   match_if flag transf prog tprog ->
@@ -436,11 +343,30 @@ Proof.
   intros. unfold match_if in *. destruct (flag tt). eauto. subst. apply forward_simulation_identity.
 Qed.
 
+Lemma exposed_match_if_injection:
+  forall (A: Type) (sem: A -> semantics)(get_mem: forall p, state (sem p) -> Memory.Mem.mem ) (flag: unit -> bool) (transf: A -> A -> Prop) (prog tprog: A),
+  match_if flag transf prog tprog ->
+  (forall p tp, transf p tp -> forward_injection (sem p) (sem tp) (get_mem p) (get_mem tp)) ->
+  forward_injection (sem prog) (sem tprog) (get_mem prog) (get_mem tprog).
+Proof.
+  intros. unfold match_if in *. destruct (flag tt). eauto. subst.
+  apply forward_injection_identity.
+Qed.
+
+Lemma exposed_match_if_extension:
+  forall (A: Type) (sem: A -> semantics)(get_mem: forall p, state (sem p) -> Memory.Mem.mem ) (flag: unit -> bool) (transf: A -> A -> Prop) (prog tprog: A),
+  match_if flag transf prog tprog ->
+  (forall p tp, transf p tp -> forward_extension (sem p) (sem tp) (get_mem p) (get_mem tp)) ->
+  forward_extension (sem prog) (sem tprog) (get_mem prog) (get_mem tprog).
+Proof.
+  intros. unfold match_if in *. destruct (flag tt). eauto. subst.
+  apply forward_extension_identity.
+Qed.
 
 Theorem simpl_clight_semantic_preservation:
   forall p tp,
   simpl_match_prog p tp ->
-  forward_simulation (Clight.semantics2 p) (Asm.semantics tp).
+  forward_injection (Clight.semantics2 p) (Asm.semantics tp) Clight.get_mem Asm.get_mem.
 Proof.
   intros p tp M. unfold simpl_match_prog, pass_match in M; simpl in M.
 Ltac DestructM' :=
@@ -450,131 +376,57 @@ Ltac DestructM' :=
       destruct H as (p & M & MM); clear H
   end.
   repeat DestructM'. subst tp.
-  assert (F: forward_simulation (Clight.semantics2 p) (Asm.semantics p19)).
-  {
-   eapply compose_forward_simulations.
-    eapply Cshmgenproof.transl_program_correct; eassumption.
-  eapply compose_forward_simulations.
-    eapply Cminorgenproof.transl_program_correct; eassumption.
-  eapply compose_forward_simulations.
-    eapply Selectionproof.transf_program_correct; eassumption.
-  eapply compose_forward_simulations.
-    eapply RTLgenproof.transf_program_correct; eassumption.
-  eapply compose_forward_simulations.
-    eapply match_if_simulation. eassumption. exact Tailcallproof.transf_program_correct.
-  eapply compose_forward_simulations.
-    eapply Inliningproof.transf_program_correct; eassumption.
-  eapply compose_forward_simulations. eapply Renumberproof.transf_program_correct; eassumption.
-  eapply compose_forward_simulations.
-    eapply match_if_simulation. eassumption. exact Constpropproof.transf_program_correct.
-  eapply compose_forward_simulations.
-    eapply match_if_simulation. eassumption. exact Renumberproof.transf_program_correct.
-  eapply compose_forward_simulations.
-    eapply match_if_simulation. eassumption. exact CSEproof.transf_program_correct.
-  eapply compose_forward_simulations.
-    eapply match_if_simulation. eassumption. exact Deadcodeproof.transf_program_correct; eassumption.
-  eapply compose_forward_simulations.
-    eapply Unusedglobproof.transf_program_correct; eassumption.
-  eapply compose_forward_simulations.
-    eapply Allocproof.transf_program_correct; eassumption.
-  eapply compose_forward_simulations.
-    eapply Tunnelingproof.transf_program_correct; eassumption.
-  eapply compose_forward_simulations.
-    eapply Linearizeproof.transf_program_correct; eassumption.
-  eapply compose_forward_simulations.
-    eapply CleanupLabelsproof.transf_program_correct; eassumption.
-  eapply compose_forward_simulations.
-    eapply match_if_simulation. eassumption. exact Debugvarproof.transf_program_correct.
-  eapply compose_forward_simulations.
-    eapply Stackingproof.transf_program_correct with (return_address_offset := Asmgenproof0.return_address_offset).
+   eapply extension_injection_composition.
+    eapply Cshmgenproof.exposed_transl_program_correct; eassumption.
+  eapply injection_injection_composition.
+    eapply Cminorgenproof.exposed_transl_program_correct; eassumption.
+  eapply extension_injection_composition.
+    eapply Selectionproof.exposed_transl_program_correct; eassumption.
+  eapply extension_injection_composition.
+    eapply RTLgenproof.exposed_transl_program_correct; eassumption.
+  eapply extension_injection_composition with (L2:=RTL.semantics p5).
+    eapply (exposed_match_if_extension _ RTL.semantics ( fun _ => RTL.get_mem)); eauto.
+    eexact Tailcallproof.exposed_transl_program_correct. 
+  eapply extension_injection_composition.
+    eapply Renumberproof.exposed_transl_program_correct; eassumption.
+  eapply extension_injection_composition.
+    eapply (exposed_match_if_extension _ RTL.semantics ( fun _ => RTL.get_mem)); eauto.
+    exact Constpropproof.exposed_transl_program_correct.
+  eapply extension_injection_composition.
+    eapply (exposed_match_if_extension _ RTL.semantics ( fun _ => RTL.get_mem)); eauto.
+    exact Renumberproof.exposed_transl_program_correct.
+  eapply extension_injection_composition.
+    eapply (exposed_match_if_extension _ RTL.semantics ( fun _ => RTL.get_mem)); eauto.
+    exact CSEproof.exposed_transl_program_correct.
+  eapply extension_injection_composition.
+    eapply Allocproof.exposed_transl_program_correct; eassumption.
+  eapply extension_injection_composition.
+    eapply Tunnelingproof.exposed_transl_program_correct; eassumption.
+  eapply extension_injection_composition.
+    eapply Linearizeproof.exposed_transl_program_correct; eassumption.
+  eapply extension_injection_composition.
+    eapply CleanupLabelsproof.exposed_transl_program_correct; eassumption.
+  eapply extension_injection_composition.
+    eapply (exposed_match_if_extension _ Linear.semantics ( fun _ => Linear.get_mem)); eauto.
+    exact Debugvarproof.exposed_transl_program_correct.
+  eapply injection_extension_composition.
+    Axiom Stackingproof_exposed_transl_program_correct:
+      forall prog return_address_offset tprog,
+        forall (return_address_offset_exists:
+             forall f sg ros c,
+               is_tail (Mach.Mcall sg ros :: c) (Mach.fn_code f) ->
+               exists ofs, return_address_offset f c ofs),
+       Stackingproof_temp.match_prog prog tprog->
+       forward_injection (Linear.semantics prog)
+                         (Mach.semantics return_address_offset tprog)
+                         Linear.get_mem Mach.get_mem.
+    eapply Stackingproof_exposed_transl_program_correct with (return_address_offset:= Asmgenproof0.return_address_offset).
     exact Asmgenproof.return_address_exists.
     eassumption.
-  eapply Asmgenproof.transf_program_correct; eassumption.
-  }
-  auto.
+    eapply Asmgenproof.exposed_transf_program_correct; eassumption.
+  
 Qed.
 
-
-Theorem cstrategy_semantic_preservation:
-  forall p tp,
-  match_prog p tp ->
-  forward_simulation (Cstrategy.semantics p) (Asm.semantics tp)
-  /\ backward_simulation (atomic (Cstrategy.semantics p)) (Asm.semantics tp).
-Proof.
-  intros p tp M. unfold match_prog, pass_match in M; simpl in M.
-Ltac DestructM :=
-  match goal with
-    [ H: exists p, _ /\ _ |- _ ] => 
-      let p := fresh "p" in let M := fresh "M" in let MM := fresh "MM" in
-      destruct H as (p & M & MM); clear H
-  end.
-  repeat DestructM. subst tp.
-  assert (F: forward_simulation (Cstrategy.semantics p) (Asm.semantics p21)).
-  {
-  eapply compose_forward_simulations.
-    eapply SimplExprproof.transl_program_correct; eassumption.
-  eapply compose_forward_simulations.
-    eapply SimplLocalsproof.transf_program_correct; eassumption.
-  eapply compose_forward_simulations.
-    eapply Cshmgenproof.transl_program_correct; eassumption.
-  eapply compose_forward_simulations.
-    eapply Cminorgenproof.transl_program_correct; eassumption.
-  eapply compose_forward_simulations.
-    eapply Selectionproof.transf_program_correct; eassumption.
-  eapply compose_forward_simulations.
-    eapply RTLgenproof.transf_program_correct; eassumption.
-  eapply compose_forward_simulations.
-    eapply match_if_simulation. eassumption. exact Tailcallproof.transf_program_correct.
-  eapply compose_forward_simulations.
-    eapply Inliningproof.transf_program_correct; eassumption.
-  eapply compose_forward_simulations. eapply Renumberproof.transf_program_correct; eassumption.
-  eapply compose_forward_simulations.
-    eapply match_if_simulation. eassumption. exact Constpropproof.transf_program_correct.
-  eapply compose_forward_simulations.
-    eapply match_if_simulation. eassumption. exact Renumberproof.transf_program_correct.
-  eapply compose_forward_simulations.
-    eapply match_if_simulation. eassumption. exact CSEproof.transf_program_correct.
-  eapply compose_forward_simulations.
-    eapply match_if_simulation. eassumption. exact Deadcodeproof.transf_program_correct; eassumption.
-  eapply compose_forward_simulations.
-    eapply Unusedglobproof.transf_program_correct; eassumption.
-  eapply compose_forward_simulations.
-    eapply Allocproof.transf_program_correct; eassumption.
-  eapply compose_forward_simulations.
-    eapply Tunnelingproof.transf_program_correct; eassumption.
-  eapply compose_forward_simulations.
-    eapply Linearizeproof.transf_program_correct; eassumption.
-  eapply compose_forward_simulations.
-    eapply CleanupLabelsproof.transf_program_correct; eassumption.
-  eapply compose_forward_simulations.
-    eapply match_if_simulation. eassumption. exact Debugvarproof.transf_program_correct.
-  eapply compose_forward_simulations.
-    eapply Stackingproof.transf_program_correct with (return_address_offset := Asmgenproof0.return_address_offset).
-    exact Asmgenproof.return_address_exists.
-    eassumption.
-  eapply Asmgenproof.transf_program_correct; eassumption.
-  }
-  split. auto.
-  apply forward_to_backward_simulation.
-  apply factor_forward_simulation. auto. eapply sd_traces. eapply Asm.semantics_determinate.
-  apply atomic_receptive. apply Cstrategy.semantics_strongly_receptive.
-  apply Asm.semantics_determinate.
-Qed.
-
-Theorem c_semantic_preservation:
-  forall p tp,
-  match_prog p tp ->
-  backward_simulation (Csem.semantics p) (Asm.semantics tp).
-Proof.
-  intros.
-  apply compose_backward_simulation with (atomic (Cstrategy.semantics p)).
-  eapply sd_traces; eapply Asm.semantics_determinate.
-  apply factor_backward_simulation.
-  apply Cstrategy.strategy_simulation.
-  apply Csem.semantics_single_events.
-  eapply ssr_well_behaved; eapply Cstrategy.semantics_strongly_receptive.
-  exact (proj2 (cstrategy_semantic_preservation _ _ H)).
-Qed.
 
 (** * Correctness of the CompCert compiler *)
 
@@ -588,39 +440,11 @@ Qed.
   exists a backward simulation of the dynamic semantics of [p]
   by the dynamic semantics of [tp]. *)
 
-Theorem transf_c_program_correct:
+Theorem transf_clight_program_correct:
   forall p tp,
-  transf_c_program p = OK tp ->
-  backward_simulation (Csem.semantics p) (Asm.semantics tp).
+  simpl_transf_clight_program p = OK tp  ->
+  forward_injection (Clight.semantics2 p) (Asm.semantics tp) Clight.get_mem Asm.get_mem.
 Proof.
-  intros. apply c_semantic_preservation. apply transf_c_program_match; auto.
-Qed.
-
-(** Here is the separate compilation case.  Consider a nonempty list [c_units]
-  of C source files (compilation units), [C1 ,,, Cn].  Assume that every
-  C compilation unit [Ci] is successfully compiled by CompCert, obtaining
-  an Asm compilation unit [Ai].  Let [asm_unit] be the nonempty list
-  [A1 ... An].  Further assume that the C units [C1 ... Cn] can be linked
-  together to produce a whole C program [c_program].  Then, the generated
-  Asm units can be linked together, producing a whole Asm program
-  [asm_program].  Moreover, [asm_program] preserves the semantics of
-  [c_program], in the sense that there exists a backward simulation of
-  the dynamic semantics of [asm_program] by the dynamic semantics of [c_program].
-*)
-
-Theorem separate_transf_c_program_correct:
-  forall c_units asm_units c_program,
-  nlist_forall2 (fun cu tcu => transf_c_program cu = OK tcu) c_units asm_units ->
-  link_list c_units = Some c_program ->
-  exists asm_program, 
-      link_list asm_units = Some asm_program
-   /\ backward_simulation (Csem.semantics c_program) (Asm.semantics asm_program).
-Proof.
-  intros. 
-  assert (nlist_forall2 match_prog c_units asm_units).
-  { eapply nlist_forall2_imply. eauto. simpl; intros. apply transf_c_program_match; auto. }
-  assert (exists asm_program, link_list asm_units = Some asm_program /\ match_prog c_program asm_program).
-  { eapply link_list_compose_passes; eauto. }
-  destruct H2 as (asm_program & P & Q).
-  exists asm_program; split; auto. apply c_semantic_preservation; auto.
+  intros. apply simpl_clight_semantic_preservation.
+  apply transf_clight_program_match; auto.
 Qed.
