backend/RTLgenproof.v
@@ -1599,4 +1599,12 @@ Proof.
   - apply transl_program_correct'.
 Qed.
 
+Theorem exposed_transl_program_correct:
+  @forward_extension
+    (CminorSel.semantics prog) (RTL.semantics tprog)
+    CminorSel.get_mem RTL.get_mem.
+Proof.
+  econstructor. eapply transl_program_correct''.
+Qed.
+
 End CORRECTNESS.
